# baseURI: https://unifiedcyberontology.org/ontology/uco/tool
# imports: https://unifiedcyberontology.org/ontology/uco/core

@base <https://unifiedcyberontology.org/ontology/uco/tool> .
@prefix owl: <http://www.w3.org/2002/07/owl#> .
@prefix rdf: <http://www.w3.org/1999/02/22-rdf-syntax-ns#> .
@prefix rdfs: <http://www.w3.org/2000/01/rdf-schema#> .
@prefix tool: <https://unifiedcyberontology.org/ontology/uco/tool#> .
@prefix xsd: <http://www.w3.org/2001/XMLSchema#> .

<https://unifiedcyberontology.org/ontology/uco/tool>
	a owl:Ontology ;
	rdfs:label "uco-tool"@en ;
	owl:imports <https://unifiedcyberontology.org/ontology/uco/core> ;
	.

tool:AnalyticTool
	a owl:Class ;
	rdfs:subClassOf tool:Tool ;
	rdfs:label "AnalyticTool"@en ;
	rdfs:comment "An analytic tool is an artifact of hardware and/or software utilized to accomplish a task or purpose of explanation, interpretation or logical reasoning."@en ;
	.

tool:BuildConfigurationType
	a owl:Class ;
	rdfs:subClassOf [
		a owl:Restriction ;
		owl:onProperty tool:configurationSettingDescription ;
		owl:maxQualifiedCardinality "1"^^xsd:nonNegativeInteger ;
		owl:onDataRange xsd:string ;
	] ;
	rdfs:label "BuildConfigurationType"@en ;
	rdfs:comment "A build configuration type is a characterization of how a particular version of software can or should be built."@en ;
	.

tool:BuildFacet
	a owl:Class ;
	rdfs:subClassOf
		<https://unifiedcyberontology.org/ontology/uco/core#Facet> ,
		[
			a owl:Restriction ;
			owl:onProperty tool:buildInformation ;
			owl:onClass tool:BuildInformationType ;
			owl:maxQualifiedCardinality "1"^^xsd:nonNegativeInteger ;
		]
		;
	rdfs:label "BuildFacet"@en ;
	rdfs:comment "A build facet is a grouping of characteristics unique to a particular version of a software."@en ;
	.

tool:BuildInformationType
	a owl:Class ;
	rdfs:subClassOf
		[
			a owl:Restriction ;
			owl:onProperty tool:compilationDate ;
			owl:maxCardinality "1"^^xsd:nonNegativeInteger ;
		] ,
		[
			a owl:Restriction ;
			owl:onProperty tool:buildConfiguration ;
			owl:onClass tool:BuildConfigurationType ;
			owl:maxQualifiedCardinality "1"^^xsd:nonNegativeInteger ;
		] ,
		[
			a owl:Restriction ;
			owl:onProperty tool:buildUtility ;
			owl:onClass tool:BuildUtilityType ;
			owl:maxQualifiedCardinality "1"^^xsd:nonNegativeInteger ;
		] ,
		[
			a owl:Restriction ;
			owl:onProperty tool:buildID ;
			owl:maxQualifiedCardinality "1"^^xsd:nonNegativeInteger ;
			owl:onDataRange xsd:string ;
		] ,
		[
			a owl:Restriction ;
			owl:onProperty tool:buildLabel ;
			owl:maxQualifiedCardinality "1"^^xsd:nonNegativeInteger ;
			owl:onDataRange xsd:string ;
		] ,
		[
			a owl:Restriction ;
			owl:onProperty tool:buildOutputLog ;
			owl:maxQualifiedCardinality "1"^^xsd:nonNegativeInteger ;
			owl:onDataRange xsd:string ;
		] ,
		[
			a owl:Restriction ;
			owl:onProperty tool:buildProject ;
			owl:maxQualifiedCardinality "1"^^xsd:nonNegativeInteger ;
			owl:onDataRange xsd:string ;
		] ,
		[
			a owl:Restriction ;
			owl:onProperty tool:buildScript ;
			owl:maxQualifiedCardinality "1"^^xsd:nonNegativeInteger ;
			owl:onDataRange xsd:string ;
		] ,
		[
			a owl:Restriction ;
			owl:onProperty tool:buildVersion ;
			owl:maxQualifiedCardinality "1"^^xsd:nonNegativeInteger ;
			owl:onDataRange xsd:string ;
		]
		;
	rdfs:label "BuildInformationType"@en ;
	rdfs:comment "A build information type is a grouping of characteristics that describe how a particular version of software was converted from source code to executable code."@en ;
	.

tool:BuildUtilityType
	a owl:Class ;
	rdfs:subClassOf
		[
			a owl:Restriction ;
			owl:onProperty tool:cpeid ;
			owl:maxQualifiedCardinality "1"^^xsd:nonNegativeInteger ;
			owl:onDataRange xsd:string ;
		] ,
		[
			a owl:Restriction ;
			owl:onProperty tool:swid ;
			owl:maxQualifiedCardinality "1"^^xsd:nonNegativeInteger ;
			owl:onDataRange xsd:string ;
		] ,
		[
			a owl:Restriction ;
			owl:onProperty tool:buildUtilityName ;
			owl:onDataRange xsd:string ;
			owl:qualifiedCardinality "1"^^xsd:nonNegativeInteger ;
		]
		;
	rdfs:label "BuildUtilityType"@en ;
	rdfs:comment "A build utility type characterizes the tool used to convert from source code to executable code for a particular version of software."@en ;
	.

tool:CompilerType
	a owl:Class ;
	rdfs:subClassOf
		[
			a owl:Restriction ;
			owl:onProperty tool:compilerInformalDescription ;
			owl:maxCardinality "1"^^xsd:nonNegativeInteger ;
		] ,
		[
			a owl:Restriction ;
			owl:onProperty tool:cpeid ;
			owl:maxQualifiedCardinality "1"^^xsd:nonNegativeInteger ;
			owl:onDataRange xsd:string ;
		] ,
		[
			a owl:Restriction ;
			owl:onProperty tool:swid ;
			owl:maxQualifiedCardinality "1"^^xsd:nonNegativeInteger ;
			owl:onDataRange xsd:string ;
		]
		;
	rdfs:label "CompilerType"@en ;
	rdfs:comment "A compiler type is a grouping of characteristics unique to a specific program that translates computer code written in one programming language (the source language) into another language (the target language). Typically a program that translates source code from a high-level programming language to a lower-level language (e.g., assembly language, object code, or machine code) to create an executable program. [based on https://en.wikipedia.org/wiki/Compiler]"@en ;
	.

tool:ConfigurationSettingType
	a owl:Class ;
	rdfs:subClassOf
		[
			a owl:Restriction ;
			owl:onProperty tool:itemDescription ;
			owl:maxQualifiedCardinality "1"^^xsd:nonNegativeInteger ;
			owl:onDataRange xsd:string ;
		] ,
		[
			a owl:Restriction ;
			owl:onProperty tool:itemType ;
			owl:maxQualifiedCardinality "1"^^xsd:nonNegativeInteger ;
			owl:onDataRange xsd:string ;
		] ,
		[
			a owl:Restriction ;
			owl:onProperty tool:itemName ;
			owl:onDataRange xsd:string ;
			owl:qualifiedCardinality "1"^^xsd:nonNegativeInteger ;
		] ,
		[
			a owl:Restriction ;
			owl:onProperty tool:itemValue ;
			owl:onDataRange xsd:string ;
			owl:qualifiedCardinality "1"^^xsd:nonNegativeInteger ;
		]
		;
	rdfs:label "ConfigurationSettingType"@en ;
	rdfs:comment "A configuration setting type is a grouping of characteristics unique to a particular parameter or initial setting for the use of a tool, application, or other cyber object."@en ;
	.

tool:DefensiveTool
	a owl:Class ;
	rdfs:subClassOf tool:Tool ;
	rdfs:label "DefensiveTool"@en ;
	rdfs:comment "A defensive tool is an artifact of hardware and/or software utilized to accomplish a task or purpose of guarding."@en ;
	.

tool:DependencyType
	a owl:Class ;
	rdfs:subClassOf
		[
			a owl:Restriction ;
			owl:onProperty tool:dependencyDescription ;
			owl:cardinality "1"^^xsd:nonNegativeInteger ;
		] ,
		[
			a owl:Restriction ;
			owl:onProperty tool:dependencyType ;
			owl:maxQualifiedCardinality "1"^^xsd:nonNegativeInteger ;
			owl:onDataRange xsd:string ;
		]
		;
	rdfs:label "DependencyType"@en ;
	rdfs:comment "A dependency type is a grouping of characteristics unique to something that a tool or other software relies on to function as intended."@en ;
	.

tool:LibraryType
	a owl:Class ;
	rdfs:subClassOf
		[
			a owl:Restriction ;
			owl:onProperty tool:libraryName ;
			owl:onDataRange xsd:string ;
			owl:qualifiedCardinality "1"^^xsd:nonNegativeInteger ;
		] ,
		[
			a owl:Restriction ;
			owl:onProperty tool:libraryVersion ;
			owl:onDataRange xsd:string ;
			owl:qualifiedCardinality "1"^^xsd:nonNegativeInteger ;
		]
		;
	rdfs:label "LibraryType"@en ;
	rdfs:comment "A library type is a grouping of characteristics unique to a collection of resources incorporated into the build of a software."@en ;
	.

tool:MaliciousTool
	a owl:Class ;
	rdfs:subClassOf tool:Tool ;
	rdfs:label "MaliciousTool"@en ;
	rdfs:comment "A malicious tool is an artifact of hardware and/or software utilized to accomplish a malevolent task or purpose."@en ;
	.

tool:Tool
	a owl:Class ;
	rdfs:subClassOf
		<https://unifiedcyberontology.org/ontology/uco/core#UcoObject> ,
		[
			a owl:Restriction ;
			owl:onProperty tool:creator ;
			owl:maxQualifiedCardinality "1"^^xsd:nonNegativeInteger ;
			owl:onDataRange xsd:string ;
		] ,
		[
			a owl:Restriction ;
			owl:onProperty tool:servicePack ;
			owl:maxQualifiedCardinality "1"^^xsd:nonNegativeInteger ;
			owl:onDataRange xsd:string ;
		] ,
		[
			a owl:Restriction ;
			owl:onProperty tool:toolType ;
			owl:maxQualifiedCardinality "1"^^xsd:nonNegativeInteger ;
			owl:onDataRange xsd:string ;
		] ,
		[
			a owl:Restriction ;
			owl:onProperty tool:version ;
			owl:maxQualifiedCardinality "1"^^xsd:nonNegativeInteger ;
			owl:onDataRange xsd:string ;
		]
		;
	rdfs:label "Tool"@en ;
	rdfs:comment "A tool is an element of hardware and/or software utilized to carry out a particular function."@en ;
	.

tool:ToolConfigurationTypeFacet
	a owl:Class ;
	rdfs:subClassOf <https://unifiedcyberontology.org/ontology/uco/core#Facet> ;
	rdfs:label "ToolConfigurationTypeFacet"@en ;
	rdfs:comment "A tool configuration type facet is a grouping of characteristics unique to the instantial settings and setup of a tool."@en ;
	.

tool:buildConfiguration
	a owl:ObjectProperty ;
	rdfs:label "buildConfiguration"@en ;
	rdfs:comment "How the build utility was configured for a particular build of a particular software."@en ;
	rdfs:range tool:BuildConfigurationType ;
	.

tool:buildID
	a owl:DatatypeProperty ;
	rdfs:label "buildID"@en ;
	rdfs:comment "An externally defined unique identifier for a particular build of a software."@en ;
	rdfs:range xsd:string ;
	.

tool:buildInformation
	a owl:ObjectProperty ;
	rdfs:label "buildInformation"@en ;
	rdfs:comment "Describes how a particular tool was built."@en ;
	rdfs:range tool:BuildInformationType ;
	.

tool:buildLabel
	a owl:DatatypeProperty ;
	rdfs:label "buildLabel"@en ;
	rdfs:comment "Relevant label for a particular build of a particular software."@en ;
	rdfs:range xsd:string ;
	.

tool:buildOutputLog
	a owl:DatatypeProperty ;
	rdfs:label "buildOutputLog"@en ;
	rdfs:comment "The output log of the build process for a software."@en ;
	rdfs:range xsd:string ;
	.

tool:buildProject
	a owl:DatatypeProperty ;
	rdfs:label "buildProject"@en ;
	rdfs:comment "The project name of a build of a software."@en ;
	rdfs:range xsd:string ;
	.

tool:buildScript
	a owl:DatatypeProperty ;
	rdfs:label "buildScript"@en ;
	rdfs:comment "The actual build script for a particular build of a particular software."@en ;
	rdfs:range xsd:string ;
	.

tool:buildUtility
	a owl:ObjectProperty ;
	rdfs:label "buildUtility"@en ;
	rdfs:comment "Identifies the utility used to build a software."@en ;
	rdfs:range tool:BuildUtilityType ;
	.

tool:buildUtilityName
	a owl:DatatypeProperty ;
	rdfs:label "buildUtilityName"@en ;
	rdfs:comment "The informally defined name of the utility used to build a particular software."@en ;
	rdfs:range xsd:string ;
	.

tool:buildVersion
	a owl:DatatypeProperty ;
	rdfs:label "buildVersion"@en ;
	rdfs:comment "The appropriate version descriptor of a particular build of a particular software."@en ;
	rdfs:range xsd:string ;
	.

tool:compilationDate
	a owl:DatatypeProperty ;
	rdfs:label "compilationDate"@en ;
	rdfs:comment "The compilation date for the build of a software."@en ;
	rdfs:range xsd:dateTime ;
	.

tool:compilerInformalDescription
	a owl:DatatypeProperty ;
	rdfs:label "compilerInformalDescription"@en ;
	rdfs:comment "An informal description of a compiler."@en ;
	rdfs:range xsd:string ;
	.

tool:compilers
	a owl:ObjectProperty ;
	rdfs:label "compilers"@en ;
	rdfs:comment "The compilers utilized during a particular build of a particular software."@en ;
	rdfs:range tool:CompilerType ;
	.

tool:configurationSettingDescription
	a owl:DatatypeProperty ;
	rdfs:label "configurationSettingDescription"@en ;
	rdfs:comment "Description of the configuration settings for a particular build of a particular software."@en ;
	rdfs:range xsd:string ;
	.

tool:configurationSettings
	a owl:ObjectProperty ;
	rdfs:label "configurationSettings"@en ;
	rdfs:comment "The configuration settings for a particular build of a particular software."@en ;
	rdfs:range tool:ConfigurationSettingType ;
	.

tool:cpeid
	a owl:DatatypeProperty ;
	rdfs:label "cpeid"@en ;
	rdfs:comment "Specifies the Common Platform Enumeration identifier for the software."@en ;
	rdfs:range xsd:string ;
	.

tool:creator
	a owl:DatatypeProperty ;
	rdfs:label "creator"@en ;
	rdfs:comment "The creator organization for a particular tool."@en ;
	rdfs:range xsd:string ;
	.

tool:dependencies
	a owl:ObjectProperty ;
	rdfs:label "dependencies"@en ;
	rdfs:comment "The relevant dependencies for a tool."@en ;
	rdfs:range tool:DependencyType ;
	.

tool:dependencyDescription
	a owl:DatatypeProperty ;
	rdfs:label "dependencyDescription"@en ;
	rdfs:comment "A description of a tool dependency."@en ;
	rdfs:range xsd:string ;
	.

tool:dependencyType
	a owl:DatatypeProperty ;
	rdfs:label "dependencyType"@en ;
	rdfs:comment "The type of a tool dependency."@en ;
	rdfs:range xsd:string ;
	.

tool:itemDescription
	a owl:DatatypeProperty ;
	rdfs:label "itemDescription"@en ;
	rdfs:comment "A description of a configuration item."@en ;
	rdfs:range xsd:string ;
	.

tool:itemName
	a owl:DatatypeProperty ;
	rdfs:label "itemName"@en ;
	rdfs:comment "The name of a configuration item."@en ;
	rdfs:range xsd:string ;
	.

tool:itemType
	a owl:DatatypeProperty ;
	rdfs:label "itemType"@en ;
	rdfs:comment "The type of a configuration item."@en ;
	rdfs:range xsd:string ;
	.

tool:itemValue
	a owl:DatatypeProperty ;
	rdfs:label "itemValue"@en ;
	rdfs:comment "The value of a configuration setting instance."@en ;
	rdfs:range xsd:string ;
	.

tool:libraries
	a owl:ObjectProperty ;
	rdfs:label "libraries"@en ;
	rdfs:comment "The libraries incorporated into a particular build of a software."@en ;
	rdfs:range tool:LibraryType ;
	.

tool:libraryName
	a owl:DatatypeProperty ;
	rdfs:label "libraryName"@en ;
	rdfs:comment "The name of the library."@en ;
	rdfs:range xsd:string ;
	.

tool:libraryVersion
	a owl:DatatypeProperty ;
	rdfs:label "libraryVersion"@en ;
	rdfs:comment "The version of the library."@en ;
	rdfs:range xsd:string ;
	.

tool:references
	a owl:DatatypeProperty ;
	rdfs:label "references"@en ;
	rdfs:comment "References to information describing a particular tool."@en ;
	rdfs:range xsd:anyURI ;
	.

tool:servicePack
	a owl:DatatypeProperty ;
	rdfs:label "servicePack"@en ;
	rdfs:comment "An appropriate service pack descriptor for a particular tool."@en ;
	rdfs:range xsd:string ;
	.

tool:swid
	a owl:DatatypeProperty ;
	rdfs:label "swid"@en ;
	rdfs:comment "Specifies the SWID tag for the software."@en ;
	rdfs:range xsd:string ;
	.

tool:toolType
	a owl:DatatypeProperty ;
	rdfs:label "toolType"@en ;
	rdfs:comment "The type of tool."@en ;
	rdfs:range xsd:string ;
	.

tool:usageContextAssumptions
	a owl:DatatypeProperty ;
	rdfs:label "usageContextAssumptions"@en ;
	rdfs:comment "dDescriptions of the various relevant usage context assumptions for this tool ."@en ;
	rdfs:range xsd:string ;
	.

tool:version
	a owl:DatatypeProperty ;
	rdfs:label "version"@en ;
	rdfs:comment "An appropriate version descriptor of a particular tool."@en ;
	rdfs:range xsd:string ;
	.

